@prefix :        <https://w3id.org/vocabulary/cop#> .
@prefix rdfs:    <http://www.w3.org/2000/01/rdf-schema#> .
@prefix cpannotationschema:  <http://www.ontologydesignpatterns.org/schemas/cpannotationschema.owl#> .
@prefix dct:     <http://purl.org/dc/terms/> .
@prefix owl:     <http://www.w3.org/2002/07/owl#> .
@prefix xsd:     <http://www.w3.org/2001/XMLSchema#> .
@prefix rdf:     <http://www.w3.org/1999/02/22-rdf-syntax-ns#> .
@prefix skos:    <http://www.w3.org/2004/02/skos/core#> .
@prefix lkif-expression:  <http://www.estrellaproject.org/lkif-core/expression.owl#> .

:Evidence
      a       owl:Class ;
      rdfs:comment "Proof(s) supporting the facts described in the complaint. Possibilities of Evidence are receipt, contract, testimony, email, and photo." ;
      rdfs:label "Evidence" ;
      rdfs:subClassOf
              [ a       owl:Restriction ;
                owl:onProperty
                        [ owl:inverseOf :supportedBy
                        ] ;
                owl:someValuesFrom :Fact
              ] ;
      owl:disjointWith :Request , :Medium , :Motivation , :Fact .

dct:contibutor
      a       owl:AnnotationProperty .

:     a       owl:Ontology ;
      dct:contibutor "Pompeu Casanovas" , "Victor Rodriguez" , "Marcos Da Silveira" , "Cedric Pruski" , "Leon van der Torre" ;
      dct:creator "Cristiana Santos" ;
      dct:date "2016-04-24" ;
      dct:license <http://purl.org/NET/rdflicense/cc-by4.0> ;
      dct:rights "This ontology is distributed under a Creative Commons CC-BY 4.0 license - https://creativecommons.org/licenses/by/4.0/" ;
      dct:title "Complaint Ontology Pattern" ;
      cpannotationschema:coversRequirements
              "Which medium was used to express the complaint?" , "Which facts happened in 'this' date or in 'this' place?" , "What is the claim of the complainant?" , "Who is the complaint recipient?" , "Which facts describe the complaint?" , "Who is involved in this complaint?" , "What motivates the complaint?" , "What evidences are used to prove the narrated fact?" ;
      cpannotationschema:hasConsequences
              "Heterogeneous models for complaints can be aligned to this pattern, which then acts as a semantic facade to different complaint management applications (such as complaint handling process, customer complaint management, customer relation management)" ;
      cpannotationschema:hasIntent
              "To represent the core constituents of a complaint" ;
      cpannotationschema:scenarios
              "A complaint refers to the narrated facts of an agent, grounded with motive and a request, through a specific medium (used to generate the complaint document), where evidence may support the facts." ;
      owl:imports <http://www.ontologydesignpatterns.org/schemas/cpannotationschema.owl> .

:hasStampTime
      a       owl:DatatypeProperty ;
      rdfs:comment """This property is related to the time which a complaint, evidence, fact, motivation or request was declared or referenced. Complaint: It is related to the complaint date
Evidence: It refers to the date of presentation of evidences
Fact: It is related to the date of description of the fact
Motivation; It refers to the date of a decision to make a complaint
Request: It refers to the date of the request""" ;
      rdfs:domain
              [ a       owl:Class ;
                owl:unionOf (:Complaint :Evidence :Fact :Motivation :Request)
              ] ;
      rdfs:range xsd:dateTimeStamp .

skos:relatedMatch
      a       owl:AnnotationProperty .

:madeBy
      a       owl:ObjectProperty ;
      rdfs:comment "The property relating the Complaint and Request to an Agent. A complaint and a request are made by an agent." ;
      rdfs:domain :Complaint ;
      rdfs:label "made by" ;
      rdfs:range :Agent .

:Request
      a       owl:Class ;
      rdfs:comment "A demand, claim or remedy set by the Complainant, e.g., financial compensation, apology, response, resolution, settlement, or other action." ;
      rdfs:label "Request" .

:Complainant
      a       owl:Class ;
      rdfs:comment "Person, organization, or its representative, making a complaint (ISO 10002:2014). The Complainant may be implicit in some datasets." ;
      rdfs:label "Complainant" ;
      rdfs:subClassOf :Agent ;
      owl:equivalentClass
              [ a       owl:Restriction ;
                owl:onProperty
                        [ owl:inverseOf :madeBy
                        ] ;
                owl:someValuesFrom :Complaint
              ] .

dct:rights
      a       owl:AnnotationProperty .

:Medium
      a       owl:Class ;
      rdfs:comment "A medium is a bearer of expressions, i.e. externalized propositions. Propositions become expressions once they are externalized through some medium (LKIF imported definition). In some complaint datasets, the medium is implicit." ;
      rdfs:label "Medium" ;
      owl:disjointWith :Request , :Motivation ;
      skos:closeMatch lkif-expression:Medium .

:Complaint_Recipient
      a       owl:Class ;
      rdfs:comment "Person, organization, or its representative, receiving a complaint (ISO 10002:2014). This concept varies from the addressee, which may be the Recipient, or any other that shall receive the complaint. The Complainant Recipient may be implicit in some datasets." ;
      rdfs:label "Complaint Recipient" ;
      rdfs:subClassOf :Agent ;
      owl:equivalentClass
              [ a       owl:Restriction ;
                owl:onProperty
                        [ owl:inverseOf :addressedTo
                        ] ;
                owl:someValuesFrom :Complaint
              ] .

dct:license
      a       owl:AnnotationProperty .

:ThirdParty
      a       owl:Class ;
      rdfs:comment "Any natural persons or any legal person, who is acting, including through any person acting in his name or on his behalf, for purposes not related to the object of the complaint." ;
      rdfs:label "Third Party" ;
      rdfs:subClassOf :Agent ;
      owl:equivalentClass
              [ a       owl:Restriction ;
                owl:onProperty
                        [ owl:inverseOf :hasThirdParty
                        ] ;
                owl:someValuesFrom :Complaint
              ] .

:has_complaint_motivation
      a       owl:ObjectProperty ;
      rdfs:comment "The relation expressing the Motivation of a Complaint." ;
      rdfs:domain :Complaint ;
      rdfs:label "has complaint motivation" ;
      rdfs:range :Motivation .

dct:creator
      a       owl:AnnotationProperty .

:addressedTo
      a       owl:ObjectProperty ;
      rdfs:comment "The property describing the Agent Recipient of the Complaint or the Agent Recipient of the Request" ;
      rdfs:domain :Complaint ;
      rdfs:label "addressed to" ;
      rdfs:range :Agent .

:hasTimeOccurrence
      a       owl:DatatypeProperty ;
      rdfs:comment """It allow the description of a time period used as reference to Complaint, Evidence, Fact, Motivation, or Request.
Complaint: It is related to the period involved in the complaint
Evidence: It refers to the period that evidence was acquired
Fact: It is related to the period where the fact was observed
Motivation: It refers to the period that motivated the complaint
Request: It refers to the period that request is requered to be executed""" , "Another ODP (TimeIndexedClassification) can be used to express in more detail time related values, but the link with this ODP is out of the scope of COP and may depend on each application case." ;
      rdfs:domain
              [ a       owl:Class ;
                owl:unionOf (:Complaint :Evidence :Fact :Motivation :Request)
              ] .

dct:date
      a       owl:AnnotationProperty .

:Fact
      a       owl:Class ;
      rdfs:comment "Proposition about something described in a complaint. Facts are observed events by the complainant." ;
      rdfs:label "Fact" ;
      owl:disjointWith :Request , :Motivation .

dct:title
      a       owl:AnnotationProperty .

:Motivation
      a       owl:Class ;
      rdfs:comment "Subjective motive of dissatisfaction, justified by facts." ;
      rdfs:label "Motivation" ;
      rdfs:subClassOf
              [ a       owl:Restriction ;
                owl:onProperty :justifiedBy ;
                owl:someValuesFrom :Fact
              ] ;
      owl:disjointWith :Request .

:supportedBy
      a       owl:ObjectProperty ;
      rdfs:comment "The object property stating that a Fact is supported by an Evidence." ;
      rdfs:domain :Fact ;
      rdfs:label "supported by" ;
      rdfs:range :Evidence .

:hasThirdParty
      a       owl:ObjectProperty ;
      rdfs:comment "Property describing agents which are third parties in a complaint" ;
      rdfs:domain :Complaint ;
      rdfs:label "has third party" ;
      rdfs:range :Agent .

:basedOn
      a       owl:ObjectProperty ;
      rdfs:comment "The property declaring the Facts that are the base of a Complaint." ;
      rdfs:domain :Complaint ;
      rdfs:label "based on" ;
      rdfs:range :Fact .

:Agent
      a       owl:Class ;
      rdfs:comment "An Agent can act, i.e. play the 'actor' role wrt. an action. It is a holder for propositional attitudes. As for this definition, we have adopted LKIF definition of Agent." ;
      rdfs:label "Agent" ;
      owl:disjointWith :Evidence , :Request , :Motivation , :Complaint , :Medium , :Fact ;
      skos:relatedMatch "http://www.estrellaproject.org/lkif-core/expression.owl#Agent" .

:part_of
      a       owl:ObjectProperty ;
      rdfs:comment "A request can only exist if a complain exist" ;
      rdfs:domain :Request ;
      rdfs:label "part of" ;
      rdfs:range :Complaint .

:hasSpace
      a       owl:DatatypeProperty ;
      rdfs:comment "Another ODP (Place) can be used to express in more detail space related values, but the link with this ODP is out of the scope of COP and may depend on each application case." , """It allow the description of a place used as reference to Complaint, Evidence, Fact, Motivation, or Request.
Complaint: It is related to the place where the complaint was registered (in a midia)
Evidence: It refers to the place related to the evidences
Fact: It is related to the place where the fact was observed
Motivation; It refers to the place where the fact motivated the complaint
Request: It refers to the place were the request is requered to be executed""" ;
      rdfs:domain
              [ a       owl:Class ;
                owl:unionOf (:Complaint :Evidence :Fact :Motivation :Request)
              ] .

skos:closeMatch
      a       owl:AnnotationProperty .

:justifiedBy
      a       owl:ObjectProperty ;
      rdfs:comment "Expresses the relation between the Motivation and the Fact(s)." ;
      rdfs:domain :Motivation ;
      rdfs:label "justified by" ;
      rdfs:range :Fact .

:expressedIn
      a       owl:ObjectProperty ;
      rdfs:comment "The property that declares by which Medium the Complaint is expressed." ;
      rdfs:domain :Complaint ;
      rdfs:label "expressed in" ;
      rdfs:range :Medium .

:Complaint
      a       owl:Class ;
      rdfs:comment "This class is the cornerstone for the pattern. We defined as an expression of dissatisfaction issued by a Complainant against a Complaint-Recipient, describing the facts, motivations, where a response or resolution is explicitly or implicitly expected. The complaint entity differs from the act of complaining, which is out of the scope of this ODP , as it is out of our use-case" ;
      rdfs:label "Complaint" ;
      rdfs:subClassOf
              [ a       owl:Restriction ;
                owl:onProperty :basedOn ;
                owl:someValuesFrom :Fact
              ] ;
      rdfs:subClassOf
              [ a       owl:Restriction ;
                owl:onProperty :madeBy ;
                owl:someValuesFrom :Agent
              ] ;
      rdfs:subClassOf
              [ a       owl:Restriction ;
                owl:onProperty :addressedTo ;
                owl:someValuesFrom :Agent
              ] ;
      rdfs:subClassOf
              [ a       owl:Restriction ;
                owl:onProperty :expressedIn ;
                owl:someValuesFrom :Medium
              ] ;
      owl:disjointWith :Evidence , :Request , :Medium , :Motivation , :Fact .
