<https://w3id.org/vocabulary/cop#justifiedBy> <http://www.w3.org/2000/01/rdf-schema#domain> <https://w3id.org/vocabulary/cop#Motivation> .
<https://w3id.org/vocabulary/cop#justifiedBy> <http://www.w3.org/2000/01/rdf-schema#range> <https://w3id.org/vocabulary/cop#Fact> .
<https://w3id.org/vocabulary/cop#justifiedBy> <http://www.w3.org/2000/01/rdf-schema#comment> "Expresses the relation between the Motivation and the Fact(s)." .
<https://w3id.org/vocabulary/cop#justifiedBy> <http://www.w3.org/2000/01/rdf-schema#label> "justified by" .
<https://w3id.org/vocabulary/cop#justifiedBy> <http://www.w3.org/1999/02/22-rdf-syntax-ns#type> <http://www.w3.org/2002/07/owl#ObjectProperty> .
<https://w3id.org/vocabulary/cop#part_of> <http://www.w3.org/2000/01/rdf-schema#domain> <https://w3id.org/vocabulary/cop#Request> .
<https://w3id.org/vocabulary/cop#part_of> <http://www.w3.org/2000/01/rdf-schema#range> <https://w3id.org/vocabulary/cop#Complaint> .
<https://w3id.org/vocabulary/cop#part_of> <http://www.w3.org/2000/01/rdf-schema#comment> "A request can only exist if a complain exist" .
<https://w3id.org/vocabulary/cop#part_of> <http://www.w3.org/2000/01/rdf-schema#label> "part of" .
<https://w3id.org/vocabulary/cop#part_of> <http://www.w3.org/1999/02/22-rdf-syntax-ns#type> <http://www.w3.org/2002/07/owl#ObjectProperty> .
_:AX2dX13f03329X3aX155fe4019c3X3aXX2dX7fe1 <http://www.w3.org/2002/07/owl#inverseOf> <https://w3id.org/vocabulary/cop#supportedBy> .
<http://www.w3.org/2004/02/skos/core#relatedMatch> <http://www.w3.org/1999/02/22-rdf-syntax-ns#type> <http://www.w3.org/2002/07/owl#AnnotationProperty> .
_:AX2dX13f03329X3aX155fe4019c3X3aXX2dX7ff4 <http://www.w3.org/1999/02/22-rdf-syntax-ns#rest> _:AX2dX13f03329X3aX155fe4019c3X3aXX2dX7ff3 .
_:AX2dX13f03329X3aX155fe4019c3X3aXX2dX7ff4 <http://www.w3.org/1999/02/22-rdf-syntax-ns#first> <https://w3id.org/vocabulary/cop#Evidence> .
_:AX2dX13f03329X3aX155fe4019c3X3aXX2dX7fed <http://www.w3.org/1999/02/22-rdf-syntax-ns#rest> _:AX2dX13f03329X3aX155fe4019c3X3aXX2dX7fec .
_:AX2dX13f03329X3aX155fe4019c3X3aXX2dX7fed <http://www.w3.org/1999/02/22-rdf-syntax-ns#first> <https://w3id.org/vocabulary/cop#Fact> .
<http://purl.org/dc/terms/date> <http://www.w3.org/1999/02/22-rdf-syntax-ns#type> <http://www.w3.org/2002/07/owl#AnnotationProperty> .
<https://w3id.org/vocabulary/cop#> <http://purl.org/dc/terms/contibutor> "Leon van der Torre" .
<https://w3id.org/vocabulary/cop#> <http://www.ontologydesignpatterns.org/schemas/cpannotationschema.owl#scenarios> "A complaint refers to the narrated facts of an agent, grounded with motive and a request, through a specific medium (used to generate the complaint document), where evidence may support the facts." .
<https://w3id.org/vocabulary/cop#> <http://purl.org/dc/terms/date> "2016-04-24" .
<https://w3id.org/vocabulary/cop#> <http://www.ontologydesignpatterns.org/schemas/cpannotationschema.owl#hasConsequences> "Heterogeneous models for complaints can be aligned to this pattern, which then acts as a semantic facade to different complaint management applications (such as complaint handling process, customer complaint management, customer relation management)" .
<https://w3id.org/vocabulary/cop#> <http://www.w3.org/1999/02/22-rdf-syntax-ns#type> <http://www.w3.org/2002/07/owl#Ontology> .
<https://w3id.org/vocabulary/cop#> <http://www.ontologydesignpatterns.org/schemas/cpannotationschema.owl#hasIntent> "To represent the core constituents of a complaint" .
<https://w3id.org/vocabulary/cop#> <http://purl.org/dc/terms/title> "Complaint Ontology Pattern" .
<https://w3id.org/vocabulary/cop#> <http://purl.org/dc/terms/contibutor> "Marcos Da Silveira" .
<https://w3id.org/vocabulary/cop#> <http://www.ontologydesignpatterns.org/schemas/cpannotationschema.owl#coversRequirements> "Which facts happened in 'this' date or in 'this' place?" .
<https://w3id.org/vocabulary/cop#> <http://www.ontologydesignpatterns.org/schemas/cpannotationschema.owl#coversRequirements> "Who is involved in this complaint?" .
<https://w3id.org/vocabulary/cop#> <http://purl.org/dc/terms/creator> "Cristiana Santos" .
<https://w3id.org/vocabulary/cop#> <http://purl.org/dc/terms/contibutor> "Cedric Pruski" .
<https://w3id.org/vocabulary/cop#> <http://purl.org/dc/terms/rights> "This ontology is distributed under a Creative Commons CC-BY 4.0 license - https://creativecommons.org/licenses/by/4.0/" .
<https://w3id.org/vocabulary/cop#> <http://www.ontologydesignpatterns.org/schemas/cpannotationschema.owl#coversRequirements> "Which facts describe the complaint?" .
<https://w3id.org/vocabulary/cop#> <http://purl.org/dc/terms/license> <http://purl.org/NET/rdflicense/cc-by4.0> .
<https://w3id.org/vocabulary/cop#> <http://www.ontologydesignpatterns.org/schemas/cpannotationschema.owl#coversRequirements> "Which medium was used to express the complaint?" .
<https://w3id.org/vocabulary/cop#> <http://purl.org/dc/terms/contibutor> "Victor Rodriguez" .
<https://w3id.org/vocabulary/cop#> <http://www.w3.org/2002/07/owl#imports> <http://www.ontologydesignpatterns.org/schemas/cpannotationschema.owl> .
<https://w3id.org/vocabulary/cop#> <http://www.ontologydesignpatterns.org/schemas/cpannotationschema.owl#coversRequirements> "Who is the complaint recipient?" .
<https://w3id.org/vocabulary/cop#> <http://www.ontologydesignpatterns.org/schemas/cpannotationschema.owl#coversRequirements> "What is the claim of the complainant?" .
<https://w3id.org/vocabulary/cop#> <http://purl.org/dc/terms/contibutor> "Pompeu Casanovas" .
<https://w3id.org/vocabulary/cop#> <http://www.ontologydesignpatterns.org/schemas/cpannotationschema.owl#coversRequirements> "What evidences are used to prove the narrated fact?" .
<https://w3id.org/vocabulary/cop#> <http://www.ontologydesignpatterns.org/schemas/cpannotationschema.owl#coversRequirements> "What motivates the complaint?" .
<http://purl.org/dc/terms/license> <http://www.w3.org/1999/02/22-rdf-syntax-ns#type> <http://www.w3.org/2002/07/owl#AnnotationProperty> .
_:AX2dX13f03329X3aX155fe4019c3X3aXX2dX7ffa <http://www.w3.org/1999/02/22-rdf-syntax-ns#rest> _:AX2dX13f03329X3aX155fe4019c3X3aXX2dX7ff9 .
_:AX2dX13f03329X3aX155fe4019c3X3aXX2dX7ffa <http://www.w3.org/1999/02/22-rdf-syntax-ns#first> <https://w3id.org/vocabulary/cop#Evidence> .
<https://w3id.org/vocabulary/cop#Complaint> <http://www.w3.org/1999/02/22-rdf-syntax-ns#type> <http://www.w3.org/2002/07/owl#Class> .
<https://w3id.org/vocabulary/cop#Complaint> <http://www.w3.org/2000/01/rdf-schema#comment> "This class is the cornerstone for the pattern. We defined as an expression of dissatisfaction issued by a Complainant against a Complaint-Recipient, describing the facts, motivations, where a response or resolution is explicitly or implicitly expected. The complaint entity differs from the act of complaining, which is out of the scope of this ODP , as it is out of our use-case" .
<https://w3id.org/vocabulary/cop#Complaint> <http://www.w3.org/2000/01/rdf-schema#subClassOf> _:AX2dX13f03329X3aX155fe4019c3X3aXX2dX7fe7 .
<https://w3id.org/vocabulary/cop#Complaint> <http://www.w3.org/2000/01/rdf-schema#subClassOf> _:AX2dX13f03329X3aX155fe4019c3X3aXX2dX7fe6 .
<https://w3id.org/vocabulary/cop#Complaint> <http://www.w3.org/2000/01/rdf-schema#label> "Complaint" .
<https://w3id.org/vocabulary/cop#Complaint> <http://www.w3.org/2000/01/rdf-schema#subClassOf> _:AX2dX13f03329X3aX155fe4019c3X3aXX2dX7fe5 .
<https://w3id.org/vocabulary/cop#Complaint> <http://www.w3.org/2002/07/owl#disjointWith> <https://w3id.org/vocabulary/cop#Motivation> .
<https://w3id.org/vocabulary/cop#Complaint> <http://www.w3.org/2002/07/owl#disjointWith> <https://w3id.org/vocabulary/cop#Fact> .
<https://w3id.org/vocabulary/cop#Complaint> <http://www.w3.org/2002/07/owl#disjointWith> <https://w3id.org/vocabulary/cop#Request> .
<https://w3id.org/vocabulary/cop#Complaint> <http://www.w3.org/2002/07/owl#disjointWith> <https://w3id.org/vocabulary/cop#Evidence> .
<https://w3id.org/vocabulary/cop#Complaint> <http://www.w3.org/2002/07/owl#disjointWith> <https://w3id.org/vocabulary/cop#Medium> .
<https://w3id.org/vocabulary/cop#Complaint> <http://www.w3.org/2000/01/rdf-schema#subClassOf> _:AX2dX13f03329X3aX155fe4019c3X3aXX2dX7fe8 .
_:AX2dX13f03329X3aX155fe4019c3X3aXX2dX7fe6 <http://www.w3.org/2002/07/owl#someValuesFrom> <https://w3id.org/vocabulary/cop#Agent> .
_:AX2dX13f03329X3aX155fe4019c3X3aXX2dX7fe6 <http://www.w3.org/2002/07/owl#onProperty> <https://w3id.org/vocabulary/cop#addressedTo> .
_:AX2dX13f03329X3aX155fe4019c3X3aXX2dX7fe6 <http://www.w3.org/1999/02/22-rdf-syntax-ns#type> <http://www.w3.org/2002/07/owl#Restriction> .
_:AX2dX13f03329X3aX155fe4019c3X3aXX2dX7fdf <http://www.w3.org/2002/07/owl#someValuesFrom> <https://w3id.org/vocabulary/cop#Complaint> .
_:AX2dX13f03329X3aX155fe4019c3X3aXX2dX7fdf <http://www.w3.org/2002/07/owl#onProperty> _:AX2dX13f03329X3aX155fe4019c3X3aXX2dX7fde .
_:AX2dX13f03329X3aX155fe4019c3X3aXX2dX7fdf <http://www.w3.org/1999/02/22-rdf-syntax-ns#type> <http://www.w3.org/2002/07/owl#Restriction> .
_:AX2dX13f03329X3aX155fe4019c3X3aXX2dX7ff9 <http://www.w3.org/1999/02/22-rdf-syntax-ns#rest> _:AX2dX13f03329X3aX155fe4019c3X3aXX2dX7ff8 .
_:AX2dX13f03329X3aX155fe4019c3X3aXX2dX7ff9 <http://www.w3.org/1999/02/22-rdf-syntax-ns#first> <https://w3id.org/vocabulary/cop#Fact> .
_:AX2dX13f03329X3aX155fe4019c3X3aXX2dX7fe0 <http://www.w3.org/2002/07/owl#someValuesFrom> <https://w3id.org/vocabulary/cop#Fact> .
_:AX2dX13f03329X3aX155fe4019c3X3aXX2dX7fe0 <http://www.w3.org/2002/07/owl#onProperty> <https://w3id.org/vocabulary/cop#justifiedBy> .
_:AX2dX13f03329X3aX155fe4019c3X3aXX2dX7fe0 <http://www.w3.org/1999/02/22-rdf-syntax-ns#type> <http://www.w3.org/2002/07/owl#Restriction> .
_:AX2dX13f03329X3aX155fe4019c3X3aXX2dX7ff3 <http://www.w3.org/1999/02/22-rdf-syntax-ns#rest> _:AX2dX13f03329X3aX155fe4019c3X3aXX2dX7ff2 .
_:AX2dX13f03329X3aX155fe4019c3X3aXX2dX7ff3 <http://www.w3.org/1999/02/22-rdf-syntax-ns#first> <https://w3id.org/vocabulary/cop#Fact> .
_:AX2dX13f03329X3aX155fe4019c3X3aXX2dX7fec <http://www.w3.org/1999/02/22-rdf-syntax-ns#rest> _:AX2dX13f03329X3aX155fe4019c3X3aXX2dX7feb .
_:AX2dX13f03329X3aX155fe4019c3X3aXX2dX7fec <http://www.w3.org/1999/02/22-rdf-syntax-ns#first> <https://w3id.org/vocabulary/cop#Motivation> .
<https://w3id.org/vocabulary/cop#Fact> <http://www.w3.org/2000/01/rdf-schema#comment> "Proposition about something described in a complaint. Facts are observed events by the complainant." .
<https://w3id.org/vocabulary/cop#Fact> <http://www.w3.org/2002/07/owl#disjointWith> <https://w3id.org/vocabulary/cop#Request> .
<https://w3id.org/vocabulary/cop#Fact> <http://www.w3.org/2002/07/owl#disjointWith> <https://w3id.org/vocabulary/cop#Motivation> .
<https://w3id.org/vocabulary/cop#Fact> <http://www.w3.org/2000/01/rdf-schema#label> "Fact" .
<https://w3id.org/vocabulary/cop#Fact> <http://www.w3.org/1999/02/22-rdf-syntax-ns#type> <http://www.w3.org/2002/07/owl#Class> .
<http://purl.org/dc/terms/creator> <http://www.w3.org/1999/02/22-rdf-syntax-ns#type> <http://www.w3.org/2002/07/owl#AnnotationProperty> .
<http://purl.org/dc/terms/title> <http://www.w3.org/1999/02/22-rdf-syntax-ns#type> <http://www.w3.org/2002/07/owl#AnnotationProperty> .
<http://purl.org/dc/terms/contibutor> <http://www.w3.org/1999/02/22-rdf-syntax-ns#type> <http://www.w3.org/2002/07/owl#AnnotationProperty> .
<https://w3id.org/vocabulary/cop#basedOn> <http://www.w3.org/2000/01/rdf-schema#range> <https://w3id.org/vocabulary/cop#Fact> .
<https://w3id.org/vocabulary/cop#basedOn> <http://www.w3.org/2000/01/rdf-schema#domain> <https://w3id.org/vocabulary/cop#Complaint> .
<https://w3id.org/vocabulary/cop#basedOn> <http://www.w3.org/2000/01/rdf-schema#comment> "The property declaring the Facts that are the base of a Complaint." .
<https://w3id.org/vocabulary/cop#basedOn> <http://www.w3.org/2000/01/rdf-schema#label> "based on" .
<https://w3id.org/vocabulary/cop#basedOn> <http://www.w3.org/1999/02/22-rdf-syntax-ns#type> <http://www.w3.org/2002/07/owl#ObjectProperty> .
_:AX2dX13f03329X3aX155fe4019c3X3aXX2dX7fe5 <http://www.w3.org/2002/07/owl#someValuesFrom> <https://w3id.org/vocabulary/cop#Fact> .
_:AX2dX13f03329X3aX155fe4019c3X3aXX2dX7fe5 <http://www.w3.org/2002/07/owl#onProperty> <https://w3id.org/vocabulary/cop#basedOn> .
_:AX2dX13f03329X3aX155fe4019c3X3aXX2dX7fe5 <http://www.w3.org/1999/02/22-rdf-syntax-ns#type> <http://www.w3.org/2002/07/owl#Restriction> .
_:AX2dX13f03329X3aX155fe4019c3X3aXX2dX7fde <http://www.w3.org/2002/07/owl#inverseOf> <https://w3id.org/vocabulary/cop#hasThirdParty> .
_:AX2dX13f03329X3aX155fe4019c3X3aXX2dX7ff8 <http://www.w3.org/1999/02/22-rdf-syntax-ns#rest> _:AX2dX13f03329X3aX155fe4019c3X3aXX2dX7ff7 .
_:AX2dX13f03329X3aX155fe4019c3X3aXX2dX7ff8 <http://www.w3.org/1999/02/22-rdf-syntax-ns#first> <https://w3id.org/vocabulary/cop#Motivation> .
<https://w3id.org/vocabulary/cop#Medium> <http://www.w3.org/2004/02/skos/core#closeMatch> <http://www.estrellaproject.org/lkif-core/expression.owl#Medium> .
<https://w3id.org/vocabulary/cop#Medium> <http://www.w3.org/2000/01/rdf-schema#comment> "A medium is a bearer of expressions, i.e. externalized propositions. Propositions become expressions once they are externalized through some medium (LKIF imported definition). In some complaint datasets, the medium is implicit." .
<https://w3id.org/vocabulary/cop#Medium> <http://www.w3.org/2002/07/owl#disjointWith> <https://w3id.org/vocabulary/cop#Request> .
<https://w3id.org/vocabulary/cop#Medium> <http://www.w3.org/2002/07/owl#disjointWith> <https://w3id.org/vocabulary/cop#Motivation> .
<https://w3id.org/vocabulary/cop#Medium> <http://www.w3.org/2000/01/rdf-schema#label> "Medium" .
<https://w3id.org/vocabulary/cop#Medium> <http://www.w3.org/1999/02/22-rdf-syntax-ns#type> <http://www.w3.org/2002/07/owl#Class> .
<https://w3id.org/vocabulary/cop#Complainant> <http://www.w3.org/2000/01/rdf-schema#comment> "Person, organization, or its representative, making a complaint (ISO 10002:2014). The Complainant may be implicit in some datasets." .
<https://w3id.org/vocabulary/cop#Complainant> <http://www.w3.org/2000/01/rdf-schema#subClassOf> <https://w3id.org/vocabulary/cop#Agent> .
<https://w3id.org/vocabulary/cop#Complainant> <http://www.w3.org/2002/07/owl#equivalentClass> _:AX2dX13f03329X3aX155fe4019c3X3aXX2dX7fea .
<https://w3id.org/vocabulary/cop#Complainant> <http://www.w3.org/2000/01/rdf-schema#label> "Complainant" .
<https://w3id.org/vocabulary/cop#Complainant> <http://www.w3.org/1999/02/22-rdf-syntax-ns#type> <http://www.w3.org/2002/07/owl#Class> .
_:AX2dX13f03329X3aX155fe4019c3X3aXX2dX7ff2 <http://www.w3.org/1999/02/22-rdf-syntax-ns#rest> _:AX2dX13f03329X3aX155fe4019c3X3aXX2dX7ff1 .
_:AX2dX13f03329X3aX155fe4019c3X3aXX2dX7ff2 <http://www.w3.org/1999/02/22-rdf-syntax-ns#first> <https://w3id.org/vocabulary/cop#Motivation> .
_:AX2dX13f03329X3aX155fe4019c3X3aXX2dX7feb <http://www.w3.org/1999/02/22-rdf-syntax-ns#rest> <http://www.w3.org/1999/02/22-rdf-syntax-ns#nil> .
_:AX2dX13f03329X3aX155fe4019c3X3aXX2dX7feb <http://www.w3.org/1999/02/22-rdf-syntax-ns#first> <https://w3id.org/vocabulary/cop#Request> .
<https://w3id.org/vocabulary/cop#Complaint_Recipient> <http://www.w3.org/2000/01/rdf-schema#comment> "Person, organization, or its representative, receiving a complaint (ISO 10002:2014). This concept varies from the addressee, which may be the Recipient, or any other that shall receive the complaint. The Complainant Recipient may be implicit in some datasets." .
<https://w3id.org/vocabulary/cop#Complaint_Recipient> <http://www.w3.org/2000/01/rdf-schema#subClassOf> <https://w3id.org/vocabulary/cop#Agent> .
<https://w3id.org/vocabulary/cop#Complaint_Recipient> <http://www.w3.org/2002/07/owl#equivalentClass> _:AX2dX13f03329X3aX155fe4019c3X3aXX2dX7fe4 .
<https://w3id.org/vocabulary/cop#Complaint_Recipient> <http://www.w3.org/2000/01/rdf-schema#label> "Complaint Recipient" .
<https://w3id.org/vocabulary/cop#Complaint_Recipient> <http://www.w3.org/1999/02/22-rdf-syntax-ns#type> <http://www.w3.org/2002/07/owl#Class> .
<https://w3id.org/vocabulary/cop#Evidence> <http://www.w3.org/2000/01/rdf-schema#comment> "Proof(s) supporting the facts described in the complaint. Possibilities of Evidence are receipt, contract, testimony, email, and photo." .
<https://w3id.org/vocabulary/cop#Evidence> <http://www.w3.org/2002/07/owl#disjointWith> <https://w3id.org/vocabulary/cop#Request> .
<https://w3id.org/vocabulary/cop#Evidence> <http://www.w3.org/2002/07/owl#disjointWith> <https://w3id.org/vocabulary/cop#Motivation> .
<https://w3id.org/vocabulary/cop#Evidence> <http://www.w3.org/2002/07/owl#disjointWith> <https://w3id.org/vocabulary/cop#Medium> .
<https://w3id.org/vocabulary/cop#Evidence> <http://www.w3.org/2002/07/owl#disjointWith> <https://w3id.org/vocabulary/cop#Fact> .
<https://w3id.org/vocabulary/cop#Evidence> <http://www.w3.org/2000/01/rdf-schema#subClassOf> _:AX2dX13f03329X3aX155fe4019c3X3aXX2dX7fe2 .
<https://w3id.org/vocabulary/cop#Evidence> <http://www.w3.org/2000/01/rdf-schema#label> "Evidence" .
<https://w3id.org/vocabulary/cop#Evidence> <http://www.w3.org/1999/02/22-rdf-syntax-ns#type> <http://www.w3.org/2002/07/owl#Class> .
_:AX2dX13f03329X3aX155fe4019c3X3aXX2dX7fe4 <http://www.w3.org/2002/07/owl#someValuesFrom> <https://w3id.org/vocabulary/cop#Complaint> .
_:AX2dX13f03329X3aX155fe4019c3X3aXX2dX7fe4 <http://www.w3.org/2002/07/owl#onProperty> _:AX2dX13f03329X3aX155fe4019c3X3aXX2dX7fe3 .
_:AX2dX13f03329X3aX155fe4019c3X3aXX2dX7fe4 <http://www.w3.org/1999/02/22-rdf-syntax-ns#type> <http://www.w3.org/2002/07/owl#Restriction> .
_:AX2dX13f03329X3aX155fe4019c3X3aXX2dX7ff7 <http://www.w3.org/1999/02/22-rdf-syntax-ns#rest> <http://www.w3.org/1999/02/22-rdf-syntax-ns#nil> .
_:AX2dX13f03329X3aX155fe4019c3X3aXX2dX7ff7 <http://www.w3.org/1999/02/22-rdf-syntax-ns#first> <https://w3id.org/vocabulary/cop#Request> .
<https://w3id.org/vocabulary/cop#ThirdParty> <http://www.w3.org/2000/01/rdf-schema#comment> "Any natural persons or any legal person, who is acting, including through any person acting in his name or on his behalf, for purposes not related to the object of the complaint." .
<https://w3id.org/vocabulary/cop#ThirdParty> <http://www.w3.org/2000/01/rdf-schema#subClassOf> <https://w3id.org/vocabulary/cop#Agent> .
<https://w3id.org/vocabulary/cop#ThirdParty> <http://www.w3.org/2002/07/owl#equivalentClass> _:AX2dX13f03329X3aX155fe4019c3X3aXX2dX7fdf .
<https://w3id.org/vocabulary/cop#ThirdParty> <http://www.w3.org/2000/01/rdf-schema#label> "Third Party" .
<https://w3id.org/vocabulary/cop#ThirdParty> <http://www.w3.org/1999/02/22-rdf-syntax-ns#type> <http://www.w3.org/2002/07/owl#Class> .
<https://w3id.org/vocabulary/cop#hasSpace> <http://www.w3.org/2000/01/rdf-schema#domain> _:AX2dX13f03329X3aX155fe4019c3X3aXX2dX7ffc .
<https://w3id.org/vocabulary/cop#hasSpace> <http://www.w3.org/2000/01/rdf-schema#comment> "It allow the description of a place used as reference to Complaint, Evidence, Fact, Motivation, or Request.\nComplaint: It is related to the place where the complaint was registered (in a midia)\nEvidence: It refers to the place related to the evidences\nFact: It is related to the place where the fact was observed\nMotivation; It refers to the place where the fact motivated the complaint\nRequest: It refers to the place were the request is requered to be executed" .
<https://w3id.org/vocabulary/cop#hasSpace> <http://www.w3.org/2000/01/rdf-schema#comment> "Another ODP (Place) can be used to express in more detail space related values, but the link with this ODP is out of the scope of COP and may depend on each application case." .
<https://w3id.org/vocabulary/cop#hasSpace> <http://www.w3.org/1999/02/22-rdf-syntax-ns#type> <http://www.w3.org/2002/07/owl#DatatypeProperty> .
_:AX2dX13f03329X3aX155fe4019c3X3aXX2dX7ff1 <http://www.w3.org/1999/02/22-rdf-syntax-ns#rest> <http://www.w3.org/1999/02/22-rdf-syntax-ns#nil> .
_:AX2dX13f03329X3aX155fe4019c3X3aXX2dX7ff1 <http://www.w3.org/1999/02/22-rdf-syntax-ns#first> <https://w3id.org/vocabulary/cop#Request> .
_:AX2dX13f03329X3aX155fe4019c3X3aXX2dX7fea <http://www.w3.org/2002/07/owl#someValuesFrom> <https://w3id.org/vocabulary/cop#Complaint> .
_:AX2dX13f03329X3aX155fe4019c3X3aXX2dX7fea <http://www.w3.org/2002/07/owl#onProperty> _:AX2dX13f03329X3aX155fe4019c3X3aXX2dX7fe9 .
_:AX2dX13f03329X3aX155fe4019c3X3aXX2dX7fea <http://www.w3.org/1999/02/22-rdf-syntax-ns#type> <http://www.w3.org/2002/07/owl#Restriction> .
<https://w3id.org/vocabulary/cop#hasStampTime> <http://www.w3.org/2000/01/rdf-schema#domain> _:AX2dX13f03329X3aX155fe4019c3X3aXX2dX7ff6 .
<https://w3id.org/vocabulary/cop#hasStampTime> <http://www.w3.org/2000/01/rdf-schema#range> <http://www.w3.org/2001/XMLSchema#dateTimeStamp> .
<https://w3id.org/vocabulary/cop#hasStampTime> <http://www.w3.org/2000/01/rdf-schema#comment> "This property is related to the time which a complaint, evidence, fact, motivation or request was declared or referenced. Complaint: It is related to the complaint date\nEvidence: It refers to the date of presentation of evidences\nFact: It is related to the date of description of the fact\nMotivation; It refers to the date of a decision to make a complaint\nRequest: It refers to the date of the request" .
<https://w3id.org/vocabulary/cop#hasStampTime> <http://www.w3.org/1999/02/22-rdf-syntax-ns#type> <http://www.w3.org/2002/07/owl#DatatypeProperty> .
_:AX2dX13f03329X3aX155fe4019c3X3aXX2dX7fe9 <http://www.w3.org/2002/07/owl#inverseOf> <https://w3id.org/vocabulary/cop#madeBy> .
_:AX2dX13f03329X3aX155fe4019c3X3aXX2dX7fe3 <http://www.w3.org/2002/07/owl#inverseOf> <https://w3id.org/vocabulary/cop#addressedTo> .
<https://w3id.org/vocabulary/cop#has_complaint_motivation> <http://www.w3.org/2000/01/rdf-schema#range> <https://w3id.org/vocabulary/cop#Motivation> .
<https://w3id.org/vocabulary/cop#has_complaint_motivation> <http://www.w3.org/2000/01/rdf-schema#domain> <https://w3id.org/vocabulary/cop#Complaint> .
<https://w3id.org/vocabulary/cop#has_complaint_motivation> <http://www.w3.org/2000/01/rdf-schema#comment> "The relation expressing the Motivation of a Complaint." .
<https://w3id.org/vocabulary/cop#has_complaint_motivation> <http://www.w3.org/2000/01/rdf-schema#label> "has complaint motivation" .
<https://w3id.org/vocabulary/cop#has_complaint_motivation> <http://www.w3.org/1999/02/22-rdf-syntax-ns#type> <http://www.w3.org/2002/07/owl#ObjectProperty> .
<http://purl.org/dc/terms/rights> <http://www.w3.org/1999/02/22-rdf-syntax-ns#type> <http://www.w3.org/2002/07/owl#AnnotationProperty> .
_:AX2dX13f03329X3aX155fe4019c3X3aXX2dX7ff6 <http://www.w3.org/2002/07/owl#unionOf> _:AX2dX13f03329X3aX155fe4019c3X3aXX2dX7ff5 .
_:AX2dX13f03329X3aX155fe4019c3X3aXX2dX7ff6 <http://www.w3.org/1999/02/22-rdf-syntax-ns#type> <http://www.w3.org/2002/07/owl#Class> .
<https://w3id.org/vocabulary/cop#madeBy> <http://www.w3.org/2000/01/rdf-schema#domain> <https://w3id.org/vocabulary/cop#Complaint> .
<https://w3id.org/vocabulary/cop#madeBy> <http://www.w3.org/2000/01/rdf-schema#range> <https://w3id.org/vocabulary/cop#Agent> .
<https://w3id.org/vocabulary/cop#madeBy> <http://www.w3.org/2000/01/rdf-schema#comment> "The property relating the Complaint and Request to an Agent. A complaint and a request are made by an agent." .
<https://w3id.org/vocabulary/cop#madeBy> <http://www.w3.org/2000/01/rdf-schema#label> "made by" .
<https://w3id.org/vocabulary/cop#madeBy> <http://www.w3.org/1999/02/22-rdf-syntax-ns#type> <http://www.w3.org/2002/07/owl#ObjectProperty> .
_:AX2dX13f03329X3aX155fe4019c3X3aXX2dX7fef <http://www.w3.org/1999/02/22-rdf-syntax-ns#rest> _:AX2dX13f03329X3aX155fe4019c3X3aXX2dX7fee .
_:AX2dX13f03329X3aX155fe4019c3X3aXX2dX7fef <http://www.w3.org/1999/02/22-rdf-syntax-ns#first> <https://w3id.org/vocabulary/cop#Complaint> .
<https://w3id.org/vocabulary/cop#expressedIn> <http://www.w3.org/2000/01/rdf-schema#range> <https://w3id.org/vocabulary/cop#Medium> .
<https://w3id.org/vocabulary/cop#expressedIn> <http://www.w3.org/2000/01/rdf-schema#domain> <https://w3id.org/vocabulary/cop#Complaint> .
<https://w3id.org/vocabulary/cop#expressedIn> <http://www.w3.org/2000/01/rdf-schema#comment> "The property that declares by which Medium the Complaint is expressed." .
<https://w3id.org/vocabulary/cop#expressedIn> <http://www.w3.org/2000/01/rdf-schema#label> "expressed in" .
<https://w3id.org/vocabulary/cop#expressedIn> <http://www.w3.org/1999/02/22-rdf-syntax-ns#type> <http://www.w3.org/2002/07/owl#ObjectProperty> .
_:AX2dX13f03329X3aX155fe4019c3X3aXX2dX7ff0 <http://www.w3.org/2002/07/owl#unionOf> _:AX2dX13f03329X3aX155fe4019c3X3aXX2dX7fef .
_:AX2dX13f03329X3aX155fe4019c3X3aXX2dX7ff0 <http://www.w3.org/1999/02/22-rdf-syntax-ns#type> <http://www.w3.org/2002/07/owl#Class> .
_:AX2dX13f03329X3aX155fe4019c3X3aXX2dX7ffc <http://www.w3.org/2002/07/owl#unionOf> _:AX2dX13f03329X3aX155fe4019c3X3aXX2dX7ffb .
_:AX2dX13f03329X3aX155fe4019c3X3aXX2dX7ffc <http://www.w3.org/1999/02/22-rdf-syntax-ns#type> <http://www.w3.org/2002/07/owl#Class> .
<https://w3id.org/vocabulary/cop#Request> <http://www.w3.org/2000/01/rdf-schema#comment> "A demand, claim or remedy set by the Complainant, e.g., financial compensation, apology, response, resolution, settlement, or other action." .
<https://w3id.org/vocabulary/cop#Request> <http://www.w3.org/2000/01/rdf-schema#label> "Request" .
<https://w3id.org/vocabulary/cop#Request> <http://www.w3.org/1999/02/22-rdf-syntax-ns#type> <http://www.w3.org/2002/07/owl#Class> .
_:AX2dX13f03329X3aX155fe4019c3X3aXX2dX7fe8 <http://www.w3.org/2002/07/owl#someValuesFrom> <https://w3id.org/vocabulary/cop#Medium> .
_:AX2dX13f03329X3aX155fe4019c3X3aXX2dX7fe8 <http://www.w3.org/2002/07/owl#onProperty> <https://w3id.org/vocabulary/cop#expressedIn> .
_:AX2dX13f03329X3aX155fe4019c3X3aXX2dX7fe8 <http://www.w3.org/1999/02/22-rdf-syntax-ns#type> <http://www.w3.org/2002/07/owl#Restriction> .
<https://w3id.org/vocabulary/cop#hasThirdParty> <http://www.w3.org/2000/01/rdf-schema#domain> <https://w3id.org/vocabulary/cop#Complaint> .
<https://w3id.org/vocabulary/cop#hasThirdParty> <http://www.w3.org/2000/01/rdf-schema#range> <https://w3id.org/vocabulary/cop#Agent> .
<https://w3id.org/vocabulary/cop#hasThirdParty> <http://www.w3.org/2000/01/rdf-schema#comment> "Property describing agents which are third parties in a complaint" .
<https://w3id.org/vocabulary/cop#hasThirdParty> <http://www.w3.org/2000/01/rdf-schema#label> "has third party" .
<https://w3id.org/vocabulary/cop#hasThirdParty> <http://www.w3.org/1999/02/22-rdf-syntax-ns#type> <http://www.w3.org/2002/07/owl#ObjectProperty> .
<https://w3id.org/vocabulary/cop#Motivation> <http://www.w3.org/2000/01/rdf-schema#comment> "Subjective motive of dissatisfaction, justified by facts." .
<https://w3id.org/vocabulary/cop#Motivation> <http://www.w3.org/2002/07/owl#disjointWith> <https://w3id.org/vocabulary/cop#Request> .
<https://w3id.org/vocabulary/cop#Motivation> <http://www.w3.org/2000/01/rdf-schema#subClassOf> _:AX2dX13f03329X3aX155fe4019c3X3aXX2dX7fe0 .
<https://w3id.org/vocabulary/cop#Motivation> <http://www.w3.org/2000/01/rdf-schema#label> "Motivation" .
<https://w3id.org/vocabulary/cop#Motivation> <http://www.w3.org/1999/02/22-rdf-syntax-ns#type> <http://www.w3.org/2002/07/owl#Class> .
_:AX2dX13f03329X3aX155fe4019c3X3aXX2dX7fe2 <http://www.w3.org/2002/07/owl#someValuesFrom> <https://w3id.org/vocabulary/cop#Fact> .
_:AX2dX13f03329X3aX155fe4019c3X3aXX2dX7fe2 <http://www.w3.org/2002/07/owl#onProperty> _:AX2dX13f03329X3aX155fe4019c3X3aXX2dX7fe1 .
_:AX2dX13f03329X3aX155fe4019c3X3aXX2dX7fe2 <http://www.w3.org/1999/02/22-rdf-syntax-ns#type> <http://www.w3.org/2002/07/owl#Restriction> .
<https://w3id.org/vocabulary/cop#Agent> <http://www.w3.org/2002/07/owl#disjointWith> <https://w3id.org/vocabulary/cop#Medium> .
<https://w3id.org/vocabulary/cop#Agent> <http://www.w3.org/2002/07/owl#disjointWith> <https://w3id.org/vocabulary/cop#Evidence> .
<https://w3id.org/vocabulary/cop#Agent> <http://www.w3.org/2002/07/owl#disjointWith> <https://w3id.org/vocabulary/cop#Request> .
<https://w3id.org/vocabulary/cop#Agent> <http://www.w3.org/2002/07/owl#disjointWith> <https://w3id.org/vocabulary/cop#Complaint> .
<https://w3id.org/vocabulary/cop#Agent> <http://www.w3.org/1999/02/22-rdf-syntax-ns#type> <http://www.w3.org/2002/07/owl#Class> .
<https://w3id.org/vocabulary/cop#Agent> <http://www.w3.org/2002/07/owl#disjointWith> <https://w3id.org/vocabulary/cop#Motivation> .
<https://w3id.org/vocabulary/cop#Agent> <http://www.w3.org/2004/02/skos/core#relatedMatch> "http://www.estrellaproject.org/lkif-core/expression.owl#Agent" .
<https://w3id.org/vocabulary/cop#Agent> <http://www.w3.org/2000/01/rdf-schema#comment> "An Agent can act, i.e. play the 'actor' role wrt. an action. It is a holder for propositional attitudes. As for this definition, we have adopted LKIF definition of Agent." .
<https://w3id.org/vocabulary/cop#Agent> <http://www.w3.org/2002/07/owl#disjointWith> <https://w3id.org/vocabulary/cop#Fact> .
<https://w3id.org/vocabulary/cop#Agent> <http://www.w3.org/2000/01/rdf-schema#label> "Agent" .
<http://www.w3.org/2004/02/skos/core#closeMatch> <http://www.w3.org/1999/02/22-rdf-syntax-ns#type> <http://www.w3.org/2002/07/owl#AnnotationProperty> .
_:AX2dX13f03329X3aX155fe4019c3X3aXX2dX7ff5 <http://www.w3.org/1999/02/22-rdf-syntax-ns#rest> _:AX2dX13f03329X3aX155fe4019c3X3aXX2dX7ff4 .
_:AX2dX13f03329X3aX155fe4019c3X3aXX2dX7ff5 <http://www.w3.org/1999/02/22-rdf-syntax-ns#first> <https://w3id.org/vocabulary/cop#Complaint> .
<https://w3id.org/vocabulary/cop#supportedBy> <http://www.w3.org/2000/01/rdf-schema#domain> <https://w3id.org/vocabulary/cop#Fact> .
<https://w3id.org/vocabulary/cop#supportedBy> <http://www.w3.org/2000/01/rdf-schema#range> <https://w3id.org/vocabulary/cop#Evidence> .
<https://w3id.org/vocabulary/cop#supportedBy> <http://www.w3.org/2000/01/rdf-schema#comment> "The object property stating that a Fact is supported by an Evidence." .
<https://w3id.org/vocabulary/cop#supportedBy> <http://www.w3.org/2000/01/rdf-schema#label> "supported by" .
<https://w3id.org/vocabulary/cop#supportedBy> <http://www.w3.org/1999/02/22-rdf-syntax-ns#type> <http://www.w3.org/2002/07/owl#ObjectProperty> .
_:AX2dX13f03329X3aX155fe4019c3X3aXX2dX7fee <http://www.w3.org/1999/02/22-rdf-syntax-ns#rest> _:AX2dX13f03329X3aX155fe4019c3X3aXX2dX7fed .
_:AX2dX13f03329X3aX155fe4019c3X3aXX2dX7fee <http://www.w3.org/1999/02/22-rdf-syntax-ns#first> <https://w3id.org/vocabulary/cop#Evidence> .
<https://w3id.org/vocabulary/cop#hasTimeOccurrence> <http://www.w3.org/2000/01/rdf-schema#domain> _:AX2dX13f03329X3aX155fe4019c3X3aXX2dX7ff0 .
<https://w3id.org/vocabulary/cop#hasTimeOccurrence> <http://www.w3.org/2000/01/rdf-schema#comment> "Another ODP (TimeIndexedClassification) can be used to express in more detail time related values, but the link with this ODP is out of the scope of COP and may depend on each application case." .
<https://w3id.org/vocabulary/cop#hasTimeOccurrence> <http://www.w3.org/2000/01/rdf-schema#comment> "It allow the description of a time period used as reference to Complaint, Evidence, Fact, Motivation, or Request.\nComplaint: It is related to the period involved in the complaint\nEvidence: It refers to the period that evidence was acquired\nFact: It is related to the period where the fact was observed\nMotivation: It refers to the period that motivated the complaint\nRequest: It refers to the period that request is requered to be executed" .
<https://w3id.org/vocabulary/cop#hasTimeOccurrence> <http://www.w3.org/1999/02/22-rdf-syntax-ns#type> <http://www.w3.org/2002/07/owl#DatatypeProperty> .
_:AX2dX13f03329X3aX155fe4019c3X3aXX2dX7ffb <http://www.w3.org/1999/02/22-rdf-syntax-ns#rest> _:AX2dX13f03329X3aX155fe4019c3X3aXX2dX7ffa .
_:AX2dX13f03329X3aX155fe4019c3X3aXX2dX7ffb <http://www.w3.org/1999/02/22-rdf-syntax-ns#first> <https://w3id.org/vocabulary/cop#Complaint> .
<https://w3id.org/vocabulary/cop#addressedTo> <http://www.w3.org/2000/01/rdf-schema#domain> <https://w3id.org/vocabulary/cop#Complaint> .
<https://w3id.org/vocabulary/cop#addressedTo> <http://www.w3.org/2000/01/rdf-schema#range> <https://w3id.org/vocabulary/cop#Agent> .
<https://w3id.org/vocabulary/cop#addressedTo> <http://www.w3.org/2000/01/rdf-schema#comment> "The property describing the Agent Recipient of the Complaint or the Agent Recipient of the Request" .
<https://w3id.org/vocabulary/cop#addressedTo> <http://www.w3.org/2000/01/rdf-schema#label> "addressed to" .
<https://w3id.org/vocabulary/cop#addressedTo> <http://www.w3.org/1999/02/22-rdf-syntax-ns#type> <http://www.w3.org/2002/07/owl#ObjectProperty> .
_:AX2dX13f03329X3aX155fe4019c3X3aXX2dX7fe7 <http://www.w3.org/2002/07/owl#someValuesFrom> <https://w3id.org/vocabulary/cop#Agent> .
_:AX2dX13f03329X3aX155fe4019c3X3aXX2dX7fe7 <http://www.w3.org/2002/07/owl#onProperty> <https://w3id.org/vocabulary/cop#madeBy> .
_:AX2dX13f03329X3aX155fe4019c3X3aXX2dX7fe7 <http://www.w3.org/1999/02/22-rdf-syntax-ns#type> <http://www.w3.org/2002/07/owl#Restriction> .
